Total/Stlc/Lang/Annotated/Theorems.lean
@@ -14,25 +14,69 @@ namespace Total.Stlc.Lang.Annotated
 
   namespace PrimOp
     namespace Eval₁
-      theorem deterministic: True := .intro
-      theorem progress: True := .intro
+      theorem deterministic {α: Nat} {δ: Domain α} {τ: Ty} {op: PrimOp δ τ} {args: Values δ} {t₁ t₂: Term τ}: Eval₁ op args t₁ → Eval₁ op args t₂ → t₁ = t₂
+        | .and _, .and _
+        | .or  _, .or  _
+        | .not _, .not _
+
+        | .add _, .add _
+        | .mul _, .mul _
+
+        | .eqBool  _, .eqBool  _
+        | .eqNat   _, .eqNat   _
+        | .neqBool _, .neqBool _
+        | .neqNat  _, .neqNat  _
+
+        | .lt  _, .lt  _
+        | .lte _, .lte _
+        | .gt  _, .gt  _
+        | .gte _, .gte _ => rfl
+
+      theorem progress {α: Nat} {δ: Domain α} {τ: Ty}: (op: PrimOp δ τ) → (args: Values δ) → ∃ t: Term τ, Eval₁ op args t ∧ Term.IsValue t
+        | .and, .cons (.bool lhs) (.nil (.bool rhs)) => ⟨_, .and (.cons (.bool lhs) (.nil (.bool rhs))), .value (.bool _)⟩
+        | .or , .cons (.bool lhs) (.nil (.bool rhs)) => ⟨_, .or  (.cons (.bool lhs) (.nil (.bool rhs))), .value (.bool _)⟩
+        | .not, .nil  (.bool op)                     => ⟨_, .not (.nil (.bool op)), .value (.bool _)⟩
+
+        | .add, .cons (.nat lhs) (.nil (.nat rhs)) => ⟨_, .add (.cons (.nat lhs) (.nil (.nat rhs))), .value (.nat _)⟩
+        | .mul, .cons (.nat lhs) (.nil (.nat rhs)) => ⟨_, .mul (.cons (.nat lhs) (.nil (.nat rhs))), .value (.nat _)⟩
+
+        | .eq,  .cons (.bool lhs) (.nil (.bool rhs)) => ⟨_, .eqBool  (.cons (.bool lhs) (.nil (.bool rhs))), .value (.bool _)⟩
+        | .eq,  .cons (.nat  lhs) (.nil (.nat  rhs)) => ⟨_, .eqNat   (.cons (.nat  lhs) (.nil (.nat  rhs))), .value (.bool _)⟩
+        | .neq, .cons (.bool lhs) (.nil (.bool rhs)) => ⟨_, .neqBool (.cons (.bool lhs) (.nil (.bool rhs))), .value (.bool _)⟩
+        | .neq, .cons (.nat  lhs) (.nil (.nat  rhs)) => ⟨_, .neqNat  (.cons (.nat  lhs) (.nil (.nat  rhs))), .value (.bool _)⟩
+
+        | .lt , .cons (.nat lhs) (.nil (.nat rhs)) => ⟨_, .lt  (.cons (.nat lhs) (.nil (.nat rhs))), .value (.bool _)⟩
+        | .lte, .cons (.nat lhs) (.nil (.nat rhs)) => ⟨_, .lte (.cons (.nat lhs) (.nil (.nat rhs))), .value (.bool _)⟩
+        | .gt , .cons (.nat lhs) (.nil (.nat rhs)) => ⟨_, .gt  (.cons (.nat lhs) (.nil (.nat rhs))), .value (.bool _)⟩
+        | .gte, .cons (.nat lhs) (.nil (.nat rhs)) => ⟨_, .gte (.cons (.nat lhs) (.nil (.nat rhs))), .value (.bool _)⟩
 
       theorem preservesHalting: True := .intro
       theorem preservesTotality: True := .intro
     end Eval₁
   end PrimOp
 
+  mutual
+    theorem Term.Eval₁.deterministic {τ: Ty} {t t₁ t₂: Term τ}: Term.Eval₁ t t₁ → Term.Eval₁ t t₂ → t₁ = t₂ := sorry
+    theorem Args.Eval₁.deterministic {α: Nat} {δ: Domain α} {a a₁ a₂: Args δ}: Args.Eval₁ a a₁ → Args.Eval₁ a a₂ → a₁ = a₂ := sorry
+  end
+
+  mutual
+    theorem Term.Eval₁.progress {τ: Ty}: (t₁: Term τ) → Term.IsValue t₁ ∨ ∃ t₂: Term τ, Term.Eval₁ t₁ t₂ := sorry
+    theorem Args.Eval₁.progress {α: Nat} {δ: Domain α}: (a₁: Args δ) → Args.IsValue a₁ ∨ ∃ a₂: Args δ, Args.Eval₁ a₁ a₂ := sorry
+  end
+
+  mutual
+    theorem Term.Eval₁.preservesHalting {τ: Ty} {t₁ t₂: Term τ} (he: Term.Eval₁ t₁ t₂): Term.Halts t₁ ↔ Term.Halts t₂ := sorry
+    theorem Args.Eval₁.preservesHalting {α: Nat} {δ: Domain α} {a₁ a₂: Args δ} (he: Args.Eval₁ a₁ a₂): Args.Halts a₁ ↔ Args.Halts a₂ := sorry
+  end
+
+  mutual
+    theorem Term.Eval₁.preservesTotality {τ: Ty} {t₁ t₂: Term τ} (he: Term.Eval₁ t₁ t₂): Term.Total t₁ ↔ Term.Total t₂ := sorry
+    theorem Args.Eval₁.preservesTotality {α: Nat} {δ: Domain α} {a₁ a₂: Args δ} (he: Args.Eval₁ a₁ a₂): Args.Total a₁ ↔ Args.Total a₂ := sorry
+  end
+
   namespace Term
-    namespace Eval₁
-      theorem deterministic {τ: Ty} {t t₁ t₂: Term τ}: Eval₁ t t₁ → Eval₁ t t₂ → t₁ = t₂ := sorry
-      theorem progress {τ: Ty} {t₁: Term τ}: IsValue t₁ ∨ ∃ t₂: Term τ, Eval₁ t₁ t₂ := sorry
-
-      theorem preservesHalting {τ: Ty} {t₁ t₂: Term τ} (he: Eval₁ t₁ t₂): Halts t₁ ↔ Halts t₂ := sorry
-      theorem preservesTotality {τ: Ty} {t₁ t₂: Term τ} (he: Eval₁ t₁ t₂): Total t₁ ↔ Total t₂ := sorry
-    end Eval₁
-
     namespace Eval
-      theorem deterministic {τ: Ty} {t t₁ t₂: Term τ}: Eval₁ t t₁ → Eval₁ t t₂ → t₁ = t₂ := sorry
       theorem progress {τ: Ty} {t₁: Term τ}: IsValue t₁ ∨ ∃ t₂: Term τ, Eval₁ t₁ t₂ := sorry
 
       theorem preservesTotality {τ: Ty} {t₁ t₂: Term τ} (he: Eval t₁ t₂): Total t₁ ↔ Total t₂ := sorry
